.

FormaleSystemeInLean/LectureAndExercise/lecture1.lean
@@ -28,9 +28,63 @@ instance : HasSSubset (Set α) where
 instance : SDiff (Set α) where
   sdiff A B := fun e => e ∈ A ∧ ¬(e ∈ B)
 
+def Set.compl (A : Set α) : Set α :=
+  fun e => ¬(e ∈ A)
+
+
 -- Set extensionality: Two sets are equal if they contain the same elements. This is not something we define but we can prove it!
 theorem Set.ext (X Y : Set α) : (∀ e, e ∈ X ↔ e ∈ Y) -> X = Y := by
   intro h; apply funext; intro e; apply propext; specialize h e; exact h
+
+
+-- TO DO: für Mengen
+/-
+- kommutativiät von ∩, ∪
+- distributivgesetze
+- de morgansche regeln
+-/
+
+theorem Set.inter_commutative (X Y : Set α) : X ∩ Y = Y ∩ X := by
+  apply Set.ext
+  intro e
+  constructor
+  . intro e_mem
+    constructor
+    . rcases e_mem with ⟨e_x, e_y⟩
+      exact e_y
+    . rcases e_mem with ⟨e_x, e_y⟩
+      exact e_x
+  . intro e_mem
+    constructor
+    . rcases e_mem with ⟨e_x, e_y⟩
+      exact e_y
+    . rcases e_mem with ⟨e_x, e_y⟩
+      exact e_x
+
+theorem Set.union_commutative (X Y : Set α) : X ∪ Y = Y ∪ X := by
+  sorry
+
+open Classical
+
+theorem Set.de_morgan1 (X Y : Set α) : X ∩ Y = (X.compl ∪ Y.compl).compl := by
+  apply Set.ext
+  intro e
+  constructor
+  . intro e_mem
+    unfold Set.compl
+    rcases e_mem with ⟨hx, hy⟩
+    intro e_n
+    rcases e_n
+    . contradiction
+    . contradiction
+  . unfold Set.compl
+    intro e_mem
+    constructor
+    .
+
+      sorry
+    .
+      sorry
 
 -- From now on, we pick some alphabet Sigma. In fact, we do not even care about the type of Sigma. In can basically be anything.
 variable {Sigma : Type u}
@@ -47,26 +101,22 @@ def Alphabet : Set Char := fun σ : Char => σ = 'a' ∨ σ = 'b'
 instance : Mul (Word Sigma) where
   mul u v := List.append u v
 
-instance [BEq Sigma] : HMul Sigma (Word Sigma) (Word Sigma) where
-  hMul σ w := List.insert σ w
+/-instance [BEq Sigma] : HMul Sigma (Word Sigma) (Word Sigma) where
+  hMul σ w := List.insert σ w -/
 
 -- Examples
 #eval ['a','b'] * ['b','a']
 
 def some_word : Word Char := ['S','t','a','u','b','e','c','k','e','n']
+def another_word : Word Char := ['A','l','t','b','a','u','c','h','a','r','m','e']
 
 #eval List.IsPrefix ['S','t','a','u','b'] some_word
---#eval List.IsInfix ['t','a','u','b'] some_word
+---#eval List.IsInfix ['t','a','u','b'] some_word
 #eval List.IsSuffix ['e','c','k','e','n'] some_word
 
 #eval 'a'::some_word
 #eval some_word.splitAt 1
 #eval some_word.append []
-
-theorem nonempty_prefix [BEq Sigma] (σ : Sigma) (w : Word Sigma) : σ::w = σ * w := by
-
-  sorry
-
 
 -- For every alphabet Sigma, there is an empty word ε. As we defined words as Lists
 -- with elements of type Sigma, ε is just the empty list [].
@@ -110,14 +160,8 @@ def L_eps : Language Sigma := fun w => w = []
 theorem sigma_star_subset : ∀ (L : Language Sigma), L ⊆ sigma_star := by
   intro L
   unfold sigma_star
-
-  have all_words : ∀ (w : Word Sigma), w ∈ sigma_star := by
-    intro w
-    unfold sigma_star
-    trivial
-
-
-  sorry
+  intro w w_mem
+  trivial
 
 -- The empty language is a subset of any language.
 theorem L_eps_subset : ∀ (L : Language Sigma), L_empty ⊆ L := by
@@ -134,7 +178,8 @@ instance : Mul (Language Sigma) where
 def Language.complement (L : Language Sigma) : Language Sigma :=
   sigma_star \ L
 
-theorem comp_via_inter (L₁ L₂ : Language Sigma) : L₁ \ L₂ = L₁ ∩ L₂.complement := by
+-- The difference between two languages can be expressed with intersection and complement.
+theorem diff_via_inter (L₁ L₂ : Language Sigma) : L₁ \ L₂ = L₁ ∩ L₂.complement := by
   apply Set.ext
   intro w
   constructor
@@ -162,3 +207,140 @@ instance : NatPow (Language Sigma) where
 -- Finally we define the Kleene Star and notation for it.
 def Language.kstar (L : Language Sigma) : Language Sigma := fun w => ∃ n, w ∈ L^n
 postfix:max "*" => Language.kstar
+
+-- Additionally, one can define a "⁺" operator which is basically the Kleene Star without n=0.
+def Language.plus (L : Language Sigma) : Language Sigma := fun w => ∃ n > 0, w ∈ L^n
+postfix:max "⁺" => Language.plus
+
+theorem split_word (w : Word Sigma) : w = u*v ↔ ∃ l : (List (Word Sigma)), l = [u, v] ∧ w = l.flatten := by
+  constructor
+  . intro w_eq
+    simp
+    exact w_eq
+  . intro l
+    rcases l with ⟨l, l_eq⟩
+    . rcases l_eq with ⟨l_eq, w_eq⟩
+      cases l_eq
+      cases w_eq
+      simp
+      trivial
+
+theorem concat_split (w : Word Sigma) : w = u*v ↔ w = [u, v].flatten := by
+  constructor
+  . intro w_eq
+    simp
+    exact w_eq
+  . intro w_eq
+    rcases w_eq
+    simp
+    trivial
+
+theorem Language.mem_pow (L : Language Sigma) (w : Word Sigma) : w ∈ L^n ↔ ∃ l : (List (Word Sigma)), w = l.flatten ∧ l.length = n ∧ (∀ u ∈ l, u ∈ L) := by
+  constructor
+  intro w_mem
+  . induction n with
+    | zero =>
+      apply Exists.intro []
+      simp
+      trivial
+    | succ n ih =>
+      rcases w_mem with ⟨v, v_mem, x, x_mem, w_eq⟩
+      constructor
+      .
+        sorry
+      .
+        sorry
+  . intro l
+    rcases l with ⟨l, hw, wl, u⟩
+
+
+    sorry
+
+
+-- TO DO: rechenregeln für sprachen
+/-
+- distributivgesetze */∪
+- {ε} neutral für *
+- K⁺ = K * K* = K* * K
+- K* = K⁺ ∪ {ε} = (K\{e}})*
+-/
+
+theorem distr_concat_union (L₁ L₂ L₃ : Language Sigma) : L₁ * (L₂ ∪ L₃) = (L₁ * L₂) ∪ (L₁ * L₃) := by
+  apply Set.ext
+  intro w
+  constructor
+  . intro w_mem
+    rcases w_mem with ⟨v, v_mem, x, x_mem, w_eq⟩
+    cases x_mem with
+    | inl x_mem =>
+      apply Or.inl
+      exists v
+      constructor
+      . exact v_mem
+      . exists x
+    | inr x_mem =>
+      apply Or.inr
+      exists v
+      constructor
+      exact v_mem
+      exists x
+  . intro w_mem
+    rcases w_mem with ⟨v, v_mem, x, x_mem, w_eq⟩
+
+    sorry
+    .
+      sorry
+
+theorem L_eps_mul : ∀ (L : Language Sigma), L ≠ L_empty → L_eps * L = L := by
+  intro L ln
+  apply Set.ext
+  intro w
+  constructor
+  . intro w_mem
+    rcases w_mem with ⟨v, v_mem, u, u_mem, _, _⟩
+    unfold L_eps at v_mem
+    cases v_mem
+    rw [concat_epsilon]
+    exact u_mem
+  . intro w_mem
+    unfold L_eps
+
+    sorry
+
+theorem mul_L_eps : ∀ (L : Language Sigma), L * L_eps = L := by
+  sorry
+
+-- The empty language ∅ is an annihilating element for concatenation.
+-- Since concatenation is not a commutative operation, we need a proof for ∅ * l = ∅ and for L * ∅ = ∅:
+theorem empty_mul : ∀ (L : Language Sigma), L_empty * L = L_empty := by
+  intro L
+  unfold L_empty
+  apply funext
+  intro w
+  simp
+  intro h
+  rcases h with ⟨u, u_mem, v, v_mem, h⟩
+  contradiction
+
+theorem mul_empty : ∀ (L : Language Sigma), L * L_empty = L_empty := by
+  intro L
+  unfold L_empty
+  apply funext
+  intro w
+  simp
+  intro h
+  rcases h with ⟨u, u_mem, v, v_mem, h⟩
+  contradiction
+
+-- All powers of ∅ (except ∅⁰) are ∅.
+theorem succ_pow_empty : ∀ n, n > 0 → Language.pow L_empty n = @L_empty Sigma := by
+  intro n n₁
+  unfold Language.pow
+  cases n₁ with
+  | refl =>
+    simp
+    unfold L_empty
+    apply empty_mul
+  | step =>
+    simp
+    apply empty_mul
